

Covariance Algebra and Inference Foundations

Linear Gaussian Models

Sai Sampath Kedari

sampath@umich.edu

Contents

1	Properties of Variance and Covariance	2
1.1	Variance	2
1.2	Covariance	2
1.3	Covariance with a Constant	2
1.4	Shift Property	2
1.5	Scaling Property	2
1.6	Symmetry of Covariance	2
1.7	Variance of a Sum	3
1.8	Variance of Linear Combination	3
1.9	Covariance of Sums	3
1.10	Multiple Random Variables	3
1.11	Covariance of Random Vectors	4
1.12	Symmetry of Covariance for Random Vectors	4
1.13	Variance of Linear Transformation	4
1.14	Affine Transformation	4
2	Joint and Marginal Gaussian Distributions	5
2.1	Marginal Gaussian Distributions	5
3	Conditional Distribution of a Jointly Gaussian Random Vector	6
3.1	Lemma 1: Joint Gaussian Density	6
3.2	Lemma 2: Conditional Density	6
3.3	Lemma 3: Block Matrix Inversion via Schur Complement	6
3.4	Applying Lemma 3 to the Covariance Matrix	6
3.5	Expansion of the Joint Quadratic Form	7
3.6	Completing the Square	7
3.7	Conditional Distribution	7

1 Properties of Variance and Covariance

Let X, Y be random variables.

1.1 Variance

$$\begin{aligned}\text{Var}(X) &= \mathbb{E}[(X - \mathbb{E}[X])^2] \\ &= \mathbb{E}[X^2 - 2X\mathbb{E}[X] + (\mathbb{E}[X])^2] \\ &= \mathbb{E}[X^2] - 2\mathbb{E}[X]\mathbb{E}[X] + (\mathbb{E}[X])^2 \\ &= \mathbb{E}[X^2] - (\mathbb{E}[X])^2\end{aligned}$$

1.2 Covariance

$$\begin{aligned}\text{Cov}(X, Y) &= \mathbb{E}[(X - \mathbb{E}[X])(Y - \mathbb{E}[Y])] \\ &= \mathbb{E}[XY - X\mathbb{E}[Y] - Y\mathbb{E}[X] + \mathbb{E}[X]\mathbb{E}[Y]] \\ &= \mathbb{E}[XY] - \mathbb{E}[X]\mathbb{E}[Y]\end{aligned}$$

1.3 Covariance with a Constant

Let c be a constant.

$$\begin{aligned}\text{Cov}(X, c) &= \mathbb{E}[(X - \mathbb{E}[X])(c - \mathbb{E}[c])] \\ &= \mathbb{E}[(X - \mathbb{E}[X]) \cdot 0] \\ &= 0\end{aligned}$$

1.4 Shift Property

$$\begin{aligned}\text{Cov}(X + c, Y) &= \mathbb{E}[(X + c - \mathbb{E}[X + c])(Y - \mathbb{E}[Y])] \\ &= \mathbb{E}[(X + c - \mathbb{E}[X] - c)(Y - \mathbb{E}[Y])] \\ &= \mathbb{E}[(X - \mathbb{E}[X])(Y - \mathbb{E}[Y])] \\ &= \text{Cov}(X, Y)\end{aligned}$$

1.5 Scaling Property

$$\begin{aligned}\text{Cov}(aX, bY) &= \mathbb{E}[(aX - \mathbb{E}[aX])(bY - \mathbb{E}[bY])] \\ &= \mathbb{E}[a(X - \mathbb{E}[X])b(Y - \mathbb{E}[Y])] \\ &= ab\mathbb{E}[(X - \mathbb{E}[X])(Y - \mathbb{E}[Y])] \\ &= ab\text{Cov}(X, Y)\end{aligned}$$

1.6 Symmetry of Covariance

$$\begin{aligned}\text{Cov}(X, Y) &= \mathbb{E}[XY] - \mathbb{E}[X]\mathbb{E}[Y] \\ &= \mathbb{E}[YX] - \mathbb{E}[Y]\mathbb{E}[X] \\ &= \text{Cov}(Y, X)\end{aligned}$$

1.7 Variance of a Sum

$$\begin{aligned}
\text{Var}(X + Y) &= \mathbb{E}[(X + Y - \mathbb{E}[X + Y])^2] \\
&= \mathbb{E}[(X - \mathbb{E}[X] + Y - \mathbb{E}[Y])^2] \\
&= \mathbb{E}[(X - \mathbb{E}[X])^2] \\
&\quad + \mathbb{E}[(Y - \mathbb{E}[Y])^2] \\
&\quad + 2\mathbb{E}[(X - \mathbb{E}[X])(Y - \mathbb{E}[Y])] \\
&= \text{Var}(X) + \text{Var}(Y) + 2\text{Cov}(X, Y)
\end{aligned}$$

1.8 Variance of Linear Combination

$$\begin{aligned}
\text{Var}(aX + bY) &= \text{Var}(aX) + \text{Var}(bY) + 2\text{Cov}(aX, bY) \\
&= a^2\text{Var}(X) + b^2\text{Var}(Y) + 2ab\text{Cov}(X, Y)
\end{aligned}$$

1.9 Covariance of Sums

$$\begin{aligned}
\text{Cov}(X + Y, Z) &= \mathbb{E}[(X + Y - \mathbb{E}[X + Y])(Z - \mathbb{E}[Z])] \\
&= \mathbb{E}[(X - \mathbb{E}[X])(Z - \mathbb{E}[Z])] \\
&\quad + \mathbb{E}[(Y - \mathbb{E}[Y])(Z - \mathbb{E}[Z])] \\
&= \text{Cov}(X, Z) + \text{Cov}(Y, Z)
\end{aligned}$$

1.10 Multiple Random Variables

Let X_1, \dots, X_m and Y_1, \dots, Y_n be random variables.

$$\begin{aligned}
\text{Cov}\left(\sum_{i=1}^m a_i X_i, \sum_{j=1}^n b_j Y_j\right) &= \mathbb{E}\left[\sum_{i=1}^m a_i (X_i - \mathbb{E}[X_i]) \sum_{j=1}^n b_j (Y_j - \mathbb{E}[Y_j])\right] \\
&= \sum_{i=1}^m \sum_{j=1}^n a_i b_j \mathbb{E}[(X_i - \mathbb{E}[X_i])(Y_j - \mathbb{E}[Y_j])] \\
&= \sum_{i=1}^m \sum_{j=1}^n a_i b_j \text{Cov}(X_i, Y_j)
\end{aligned}$$

Define the random vectors

$$\mathbf{X} = \begin{bmatrix} X_1 \\ \vdots \\ X_m \end{bmatrix}, \quad \mathbf{Y} = \begin{bmatrix} Y_1 \\ \vdots \\ Y_n \end{bmatrix},$$

and deterministic vectors

$$\mathbf{a} = \begin{bmatrix} a_1 \\ \vdots \\ a_m \end{bmatrix}, \quad \mathbf{b} = \begin{bmatrix} b_1 \\ \vdots \\ b_n \end{bmatrix}.$$

Then

$$\sum_{i=1}^m a_i X_i = \mathbf{a}^\top \mathbf{X}, \quad \sum_{j=1}^n b_j Y_j = \mathbf{b}^\top \mathbf{Y}.$$

Define the cross covariance matrix

$$\text{Cov}(\mathbf{X}, \mathbf{Y}) = \mathbb{E}[(\mathbf{X} - \mathbb{E}[\mathbf{X}])(\mathbf{Y} - \mathbb{E}[\mathbf{Y}])^\top],$$

whose (i, j) entry is $\text{Cov}(X_i, Y_j)$.

Hence,

$$\text{Cov}(\mathbf{a}^\top \mathbf{X}, \mathbf{b}^\top \mathbf{Y}) = \mathbf{a}^\top \text{Cov}(\mathbf{X}, \mathbf{Y}) \mathbf{b}.$$

1.11 Covariance of Random Vectors

Let \mathbf{X} and \mathbf{Y} be random vectors.

$$\text{Cov}(\mathbf{X}, \mathbf{Y}) = \mathbb{E}[(\mathbf{X} - \mathbb{E}[\mathbf{X}])(\mathbf{Y} - \mathbb{E}[\mathbf{Y}])^\top]$$

The covariance matrix of a random vector \mathbf{X} is defined as

$$\text{Cov}(\mathbf{X}) = \text{Cov}(\mathbf{X}, \mathbf{X}).$$

1.12 Symmetry of Covariance for Random Vectors

$$\begin{aligned} \text{Cov}(\mathbf{X}, \mathbf{Y}) &= \mathbb{E}[(\mathbf{X} - \mathbb{E}[\mathbf{X}])(\mathbf{Y} - \mathbb{E}[\mathbf{Y}])^\top] \\ &= \mathbb{E}[(\mathbf{Y} - \mathbb{E}[\mathbf{Y}])(\mathbf{X} - \mathbb{E}[\mathbf{X}])^\top]^\top \\ &= \text{Cov}(\mathbf{Y}, \mathbf{X})^\top \end{aligned}$$

1.13 Variance of Linear Transformation

Let \mathbf{x} be a random vector and A a deterministic matrix.

$$\begin{aligned} \text{Var}(A\mathbf{x}) &= \text{Cov}(A\mathbf{x}, A\mathbf{x}) \\ &= \mathbb{E}[A(\mathbf{x} - \mathbb{E}[\mathbf{x}])(\mathbf{x} - \mathbb{E}[\mathbf{x}])^\top A^\top] \\ &= A \text{Cov}(\mathbf{x}) A^\top \end{aligned}$$

1.14 Affine Transformation

Let $\mathbf{y} = A\mathbf{x} + \mathbf{b}$.

$$\begin{aligned} \text{Cov}(\mathbf{y}) &= \text{Cov}(A\mathbf{x} + \mathbf{b}, A\mathbf{x} + \mathbf{b}) \\ &= \text{Cov}(A\mathbf{x}, A\mathbf{x}) \\ &= A \text{Cov}(\mathbf{x}) A^\top \end{aligned}$$

2 Joint and Marginal Gaussian Distributions

Let

$$\mathbf{X} \in \mathbb{R}^n, \quad \mathbf{Y} \in \mathbb{R}^m$$

be random vectors with finite second moments.

Define the stacked random vector

$$\mathbf{Z} = \begin{bmatrix} \mathbf{X} \\ \mathbf{Y} \end{bmatrix} \in \mathbb{R}^{n+m}.$$

We say that (\mathbf{X}, \mathbf{Y}) is jointly Gaussian if

$$\mathbf{Z} \sim \mathcal{N}\left(\begin{bmatrix} \boldsymbol{\mu}_X \\ \boldsymbol{\mu}_Y \end{bmatrix}, \Sigma\right),$$

where

$$\Sigma = \begin{bmatrix} \Sigma_{XX} & \Sigma_{XY} \\ \Sigma_{YX} & \Sigma_{YY} \end{bmatrix}.$$

By definition of covariance for random vectors,

$$\Sigma = \mathbb{E}\left[(\mathbf{Z} - \mathbb{E}[\mathbf{Z}])(\mathbf{Z} - \mathbb{E}[\mathbf{Z}])^\top\right].$$

Expanding the outer product yields

$$\Sigma = \begin{bmatrix} \mathbb{E}\left[(\mathbf{X} - \boldsymbol{\mu}_X)(\mathbf{X} - \boldsymbol{\mu}_X)^\top\right] & \mathbb{E}\left[(\mathbf{X} - \boldsymbol{\mu}_X)(\mathbf{Y} - \boldsymbol{\mu}_Y)^\top\right] \\ \mathbb{E}\left[(\mathbf{Y} - \boldsymbol{\mu}_Y)(\mathbf{X} - \boldsymbol{\mu}_X)^\top\right] & \mathbb{E}\left[(\mathbf{Y} - \boldsymbol{\mu}_Y)(\mathbf{Y} - \boldsymbol{\mu}_Y)^\top\right] \end{bmatrix}.$$

Hence,

$$\Sigma_{XX} = \text{Cov}(\mathbf{X}), \quad \Sigma_{YY} = \text{Cov}(\mathbf{Y}), \quad \Sigma_{YX} = \Sigma_{XY}^\top.$$

2.1 Marginal Gaussian Distributions

Define the linear maps

$$A_X = \begin{bmatrix} I_n & 0 \end{bmatrix}, \quad A_Y = \begin{bmatrix} 0 & I_m \end{bmatrix}.$$

Then

$$\mathbf{X} = A_X \mathbf{Z}, \quad \mathbf{Y} = A_Y \mathbf{Z}.$$

By linearity of expectation,

$$\mathbb{E}[\mathbf{X}] = A_X \mathbb{E}[\mathbf{Z}] = \boldsymbol{\mu}_X, \quad \mathbb{E}[\mathbf{Y}] = A_Y \mathbb{E}[\mathbf{Z}] = \boldsymbol{\mu}_Y.$$

Using the covariance of a linear transformation,

$$\text{Cov}(\mathbf{X}) = A_X \Sigma A_X^\top = \Sigma_{XX}, \quad \text{Cov}(\mathbf{Y}) = A_Y \Sigma A_Y^\top = \Sigma_{YY}.$$

Hence,

$$\mathbf{X} \sim \mathcal{N}(\boldsymbol{\mu}_X, \Sigma_{XX}), \quad \mathbf{Y} \sim \mathcal{N}(\boldsymbol{\mu}_Y, \Sigma_{YY}).$$

3 Conditional Distribution of a Jointly Gaussian Random Vector

Throughout this section, we work under the joint Gaussian model defined in Section 2. We assume Σ_{YY} is symmetric positive definite.

Our goal is to derive the distribution of

$$\mathbf{X} \mid \mathbf{Y} = \mathbf{y}.$$

3.1 Lemma 1: Joint Gaussian Density

The joint density of \mathbf{Z} is

$$p(\mathbf{z}) = \frac{1}{(2\pi)^{(n+m)/2} |\Sigma|^{1/2}} \exp \left(-\frac{1}{2} (\mathbf{z} - \boldsymbol{\mu})^\top \Sigma^{-1} (\mathbf{z} - \boldsymbol{\mu}) \right).$$

3.2 Lemma 2: Conditional Density

For random vectors with joint density $p(\mathbf{x}, \mathbf{y})$,

$$p(\mathbf{x} \mid \mathbf{y}) = \frac{p(\mathbf{x}, \mathbf{y})}{p(\mathbf{y})}.$$

3.3 Lemma 3: Block Matrix Inversion via Schur Complement

Let

$$M = \begin{bmatrix} A & B \\ C & D \end{bmatrix}, \quad D \text{ invertible.}$$

Define the Schur complement

$$S = A - BD^{-1}C.$$

Assume S is invertible.

Then

$$M^{-1} = \begin{bmatrix} S^{-1} & -S^{-1}BD^{-1} \\ -D^{-1}CS^{-1} & D^{-1} + D^{-1}CS^{-1}BD^{-1} \end{bmatrix}.$$

3.4 Applying Lemma 3 to the Covariance Matrix

Identify

$$A = \Sigma_{XX}, \quad B = \Sigma_{XY}, \quad C = \Sigma_{YX}, \quad D = \Sigma_{YY}.$$

Define the conditional covariance

$$\Sigma_{X|Y} = \Sigma_{XX} - \Sigma_{XY} \Sigma_{YY}^{-1} \Sigma_{YX}.$$

Then

$$\Sigma^{-1} = \begin{bmatrix} \Sigma_{X|Y}^{-1} & -\Sigma_{X|Y}^{-1} \Sigma_{XY} \Sigma_{YY}^{-1} \\ -\Sigma_{YY}^{-1} \Sigma_{YX} \Sigma_{X|Y}^{-1} & \Sigma_{YY}^{-1} + \Sigma_{YY}^{-1} \Sigma_{YX} \Sigma_{X|Y}^{-1} \Sigma_{XY} \Sigma_{YY}^{-1} \end{bmatrix}.$$

3.5 Expansion of the Joint Quadratic Form

Define

$$Q = \begin{bmatrix} \mathbf{x} - \boldsymbol{\mu}_X \\ \mathbf{y} - \boldsymbol{\mu}_Y \end{bmatrix}^\top \Sigma^{-1} \begin{bmatrix} \mathbf{x} - \boldsymbol{\mu}_X \\ \mathbf{y} - \boldsymbol{\mu}_Y \end{bmatrix}.$$

Substituting the block inverse yields

$$\begin{aligned} Q &= (\mathbf{x} - \boldsymbol{\mu}_X)^\top \Sigma_{X|Y}^{-1} (\mathbf{x} - \boldsymbol{\mu}_X) \\ &\quad - (\mathbf{x} - \boldsymbol{\mu}_X)^\top \Sigma_{X|Y}^{-1} \Sigma_{XY} \Sigma_{YY}^{-1} (\mathbf{y} - \boldsymbol{\mu}_Y) \\ &\quad - (\mathbf{y} - \boldsymbol{\mu}_Y)^\top \Sigma_{YY}^{-1} \Sigma_{YX} \Sigma_{X|Y}^{-1} (\mathbf{x} - \boldsymbol{\mu}_X) \\ &\quad + \text{terms independent of } \mathbf{x}. \end{aligned}$$

3.6 Completing the Square

Using

$$x^\top Ax - 2x^\top b = (x - A^{-1}b)^\top A(x - A^{-1}b) - b^\top A^{-1}b,$$

define

$$\boldsymbol{\mu}_{X|Y} = \boldsymbol{\mu}_X + \Sigma_{XY} \Sigma_{YY}^{-1} (\mathbf{y} - \boldsymbol{\mu}_Y).$$

Then

$$Q = (\mathbf{x} - \boldsymbol{\mu}_{X|Y})^\top \Sigma_{X|Y}^{-1} (\mathbf{x} - \boldsymbol{\mu}_{X|Y}) + \text{terms independent of } \mathbf{x}.$$

3.7 Conditional Distribution

Therefore,

$$\mathbf{X} \mid \mathbf{Y} \sim \mathcal{N}(\boldsymbol{\mu}_{X|Y}, \Sigma_{X|Y}).$$